lean-sce/LeanSce/SCE/Syntax.lean
@@ -58,26 +58,26 @@ inductive Value : Exp → Prop where
   | vnmrg  {v₁ v₂} : Value v₁ → Value v₂ → Value (.nmrg v₁ v₂)
   | vlrec  {v l}   : Value v  → Value (.lrec l v)
 
-inductive IndexLookup : Typ → Nat → Typ → Prop
-| zero (A B : Typ) : IndexLookup (Typ.and A B) 0 B
+inductive SLookup : Typ → Nat → Typ → Prop
+| zero (A B : Typ) : SLookup (Typ.and A B) 0 B
 | succ (A B : Typ) (n : Nat) (C : Typ)
-    : IndexLookup A n C → IndexLookup (Typ.and A B) (Nat.succ n) C
+    : SLookup A n C → SLookup (Typ.and A B) (Nat.succ n) C
 
 inductive LabelIn : String -> Typ -> Prop
 | rcd (label : String) (T : Typ) : LabelIn label (Typ.rcd label T)
 | andl (A B : Typ) (label : String) : LabelIn label A → LabelIn label (Typ.and A B)
 | andr (A B : Typ) (label : String) : LabelIn label B → LabelIn label (Typ.and A B)
 
-inductive RecordLookup : Typ → String → Typ → Prop
+inductive SRLookup : Typ → String → Typ → Prop
 | zero (label : String) (T : Typ) :
-    RecordLookup (Typ.rcd label T) label T
+    SRLookup (Typ.rcd label T) label T
 | andl (A B : Typ) (label : String) (T : Typ) :
-    RecordLookup A label T →
+    SRLookup A label T →
     LabelIn label A ∧ ¬ LabelIn label B →
-    RecordLookup (Typ.and A B) label T
+    SRLookup (Typ.and A B) label T
 | andr (A B : Typ) (label : String) (T : Typ) :
-    RecordLookup B label T →
+    SRLookup B label T →
     LabelIn label B ∧ ¬ LabelIn label A →
-    RecordLookup (Typ.and A B) label T
+    SRLookup (Typ.and A B) label T
 
 end SCE
