lean-sce/LeanSce/Core/BigStep.lean
@@ -1,0 +1,72 @@
+import LeanSce.Core.Syntax
+import LeanSce.Core.Typing
+import LeanSce.Core.SmallStep
+
+open Core
+
+inductive EBig : Exp → Exp → Exp → Prop where
+  | eblit {v : Exp} {i : Nat}
+    : Value v
+    → EBig v (.lit i) (.lit i)
+  | ebunit {v : Exp}
+    : Value v
+    → EBig v .unit .unit
+  | ebmrg {v e₁ e₂ v₁ v₂ : Exp}
+    : EBig v e₁ v₁
+    → EBig (.mrg v v₁) e₂ v₂
+    → EBig v (.mrg e₁ e₂) (.mrg v₁ v₂)
+  | ebclos {v : Exp} {A : Typ} {e : Exp}
+    : Value v
+    → EBig v (.lam A e) (.clos v A e)
+  | ebapp {v e₁ e₂ v₁ v₂ vr e : Exp} {A : Typ}
+    : EBig v e₁ (.clos v₂ A e)
+    → EBig v e₂ v₁
+    → EBig (.mrg v₂ v₁) e vr
+    → EBig v (.app e₁ e₂) vr
+  | ebbox {v e₁ e₂ v₁ vr : Exp}
+    : EBig v e₁ v₁
+    → EBig v₁ e₂ vr
+    → EBig v (.box e₁ e₂) vr
+  | eclos {v v₁ : Exp} {A : Typ} {e : Exp}
+    : Value v
+    → Value v₁
+    → EBig v (.clos v₁ A e) (.clos v₁ A e)
+  | equery {e : Exp}
+    : Value e
+    → EBig e .query e
+  | ebproj {e a v v' : Exp} {n : Nat}
+    : EBig e a v
+    → LookupV v n v'
+    → EBig e (.proj a n) v'
+  | ebrec {e a v : Exp} {l : String}
+    : EBig e a v
+    → EBig e (.lrec l a) (.lrec l v)
+  | ebsel {e a v₁ v₂ : Exp} {l : String}
+    : EBig e a v₁
+    → RLookupV v₁ l v₂
+    → EBig e (.rproj a l) v₂
+
+theorem big_gpreservation
+  {e v' v : Exp}
+  (heval : EBig v e v') :
+  ∀ {E A : Typ},
+  HasType E e A
+  → HasType .top v E
+  → HasType .top v' A := by
+  sorry
+
+theorem termination
+  {E A : Typ} {e : Exp}
+  (htype : HasType E e A) :
+  ∀ {v : Exp},
+  Value v
+  → HasType .top v E
+  → ∃ v', EBig v e v' ∧ Value v' := by
+  sorry
+
+
+theorem big_preservation {e v' A}
+  : HasType .top e A
+  → EBig .unit e v'
+  → HasType .top v' A := by
+  sorry
