lean-sce/LeanSce/SCE/Elaboration.lean
@@ -1,0 +1,119 @@
+import LeanSce.SCE.Syntax
+import LeanSce.Core.Syntax
+
+open SCE
+
+mutual
+def elabTyp : Typ → Core.Typ
+  | Typ.int        => Core.Typ.int
+  | Typ.top        => Core.Typ.top
+  | Typ.arr t1 t2  => Core.Typ.arr (elabTyp t1) (elabTyp t2)
+  | Typ.and t1 t2  => Core.Typ.and (elabTyp t1) (elabTyp t2)
+  | Typ.rcd str t  => Core.Typ.rcd str (elabTyp t)
+  | Typ.sig mty    => elabModTyp mty
+
+def elabModTyp : ModTyp → Core.Typ
+  | ModTyp.TyIntf t1      => elabTyp t1
+  | ModTyp.TyArrM t1 mty  => Core.Typ.arr (elabTyp t1) (elabModTyp mty)
+end
+
+abbrev TyCtx := Typ
+
+inductive elabExp : TyCtx → Exp → Typ → Core.Exp → Prop
+  | equery {ctx}
+    : elabExp ctx Exp.query ctx Core.Exp.query
+  | elit (ctx : Typ) (n : Nat)
+    : elabExp ctx (Exp.lit n) Typ.int (Core.Exp.lit n)
+  | eunit (ctx : Typ)
+    : elabExp ctx Exp.unit Typ.top Core.Exp.unit
+  | eapp (ctx A B : Typ) (se1 se2 : Exp) (ce1 ce2 : Core.Exp)
+    : elabExp ctx se1 (Typ.arr A B) ce1
+    → elabExp ctx se2 A ce2
+    → elabExp ctx (Exp.app se1 se2) B (Core.Exp.app ce1 ce2)
+  | eproj (ctx A B : Typ) (se : Exp) (ce : Core.Exp) (i : Nat)
+    : elabExp ctx se A ce
+    → SLookup A i B
+    → elabExp ctx (Exp.proj se i) B (Core.Exp.proj ce i)
+  | ebox (ctx ctx' A : Typ) (se1 se2 : Exp) (ce1 ce2 : Core.Exp)
+    : elabExp ctx se1 ctx' ce1
+    → elabExp ctx' se2 A ce2
+    → elabExp ctx (Exp.box se1 se2) A (Core.Exp.box ce1 ce2)
+  | edmrg (ctx A B : Typ) (se1 se2 : Exp) (ce1 ce2 : Core.Exp)
+    : elabExp ctx se1 A ce1
+    → elabExp (Typ.and ctx A) se2 B ce2
+    → elabExp ctx (Exp.mrg se1 se2) (Typ.and A B) (Core.Exp.mrg ce1 ce2)
+  /-
+    Γ ⊢ eˢ₁ : A ⤳ eᶜ₁
+    Γ ⊢ eˢ₂ : B ⤳ eᶜ₂
+    ──────────────────────────────────────────────────────────
+    Γ ⊢ eˢ₁ #n eˢ₂ : A & B ⤳ (λ⟦Γ⟧. mrg (box ?.0 eᶜ₁) (box ?.1 eᶜ₂)) ?
+  -/
+  | enmrg (ctx A B : Typ) (se1 se2 : Exp) (ce1 ce2 : Core.Exp)
+    : elabExp ctx se1 A ce1
+    → elabExp ctx se2 B ce2
+    → elabExp ctx (Exp.nmrg se1 se2) (Typ.and A B)
+        (Core.Exp.app
+          (Core.Exp.lam (elabTyp ctx)
+            (Core.Exp.mrg
+              (Core.Exp.box (Core.Exp.proj Core.Exp.query 0) ce1)
+              (Core.Exp.box (Core.Exp.proj Core.Exp.query 1) ce2)))
+          Core.Exp.query)
+  | elam (ctx A B : Typ) (se : Exp) (ce : Core.Exp)
+    : elabExp (Typ.and ctx A) se B ce
+    → elabExp ctx (Exp.lam A se) (Typ.arr A B) (Core.Exp.lam (elabTyp A) ce)
+  | erproj (ctx A B : Typ) (se : Exp) (ce : Core.Exp) (l : String) :
+      elabExp ctx se B ce
+      → SRLookup B l A
+      → elabExp ctx (Exp.rproj se l) A (Core.Exp.rproj ce l)
+  | eclos (ctx ctx' A B : Typ) (se1 se2 : Exp) (ce1 ce2 : Core.Exp)
+    : SCE.Value se1
+    → elabExp Typ.top se1 ctx' ce1
+    → elabExp (Typ.and ctx' A) se2 B ce2
+    → elabExp ctx (Exp.clos se1 A se2) (Typ.arr A B) (Core.Exp.clos ce1 (elabTyp A) ce2)
+  | elrec (ctx A : Typ) (se : Exp) (ce : Core.Exp) (l : String)
+    : elabExp ctx se A ce
+    → elabExp ctx (Exp.lrec l se) (Typ.rcd l A) (Core.Exp.lrec l ce)
+  | letb (ctx A B : Typ) (se1 se2 : Exp) (ce1 ce2 : Core.Exp)
+    : elabExp ctx se1 A ce1
+    → elabExp (Typ.and ctx A) se2 B ce2
+    → elabExp ctx (Exp.letb se1 A se2) B
+        (Core.Exp.app (Core.Exp.lam (elabTyp A) ce2) ce1)
+  | openm (ctx A B : Typ) (se1 se2 : Exp) (ce1 ce2 : Core.Exp) (l : String)
+    : elabExp ctx se1 (Typ.rcd l A) ce1
+    → elabExp (Typ.and ctx A) se2 B ce2
+    → elabExp ctx (Exp.openm se1 se2) B
+        (Core.Exp.app (Core.Exp.lam (elabTyp A) ce2) (Core.Exp.rproj ce1 l))
+  | mstruct (ctx ctxInner B : Typ) (sb : Sandbox) (se : Exp) (ce envCore : Core.Exp)
+    : (sb = Sandbox.sandboxed → ctxInner = Typ.top)
+    → (sb = Sandbox.open_     → ctxInner = ctx)
+    → elabExp ctxInner se B ce
+    → elabExp ctx (Exp.mstruct sb se) (Typ.sig (ModTyp.TyIntf B))
+        (Core.Exp.box
+          (match sb with
+            | Sandbox.sandboxed => Core.Exp.unit
+            | Sandbox.open_     => Core.Exp.query)
+          ce)
+  | mfunctor (ctx ctxInner A B : Typ) (mt : ModTyp) (sb : Sandbox) (se : Exp) (ce : Core.Exp)
+    : (sb = Sandbox.sandboxed → ctxInner = Typ.and Typ.top A)
+    → (sb = Sandbox.open_     → ctxInner = Typ.and ctx A)
+    → elabExp ctxInner se B ce
+    → elabExp ctx (Exp.mfunctor sb A se) (Typ.sig mt)
+        (match sb with
+          | Sandbox.sandboxed => Core.Exp.box Core.Exp.unit (Core.Exp.lam (elabTyp A) ce)
+          | Sandbox.open_     => Core.Exp.lam (elabTyp A) ce)
+  | mclos (ctx ctx' A B : Typ) (mt : ModTyp) (se1 se2 : Exp) (ce1 ce2 : Core.Exp)
+    : SCE.Value se1
+    → elabExp Typ.top se1 ctx' ce1
+    → elabExp (Typ.and ctx' A) se2 B ce2
+    → elabExp ctx (Exp.mclos se1 A se2) (Typ.sig mt)
+        (Core.Exp.clos ce1 (elabTyp A) ce2)
+  | mapp (ctx A : Typ) (mt : ModTyp) (se1 se2 : Exp) (ce1 ce2 : Core.Exp)
+    : elabExp ctx se1 (Typ.sig (ModTyp.TyArrM A mt)) ce1
+    → elabExp ctx se2 A ce2
+    → elabExp ctx (Exp.mapp se1 se2) (Typ.sig mt)
+        (Core.Exp.app ce1 ce2)
+  | mlink (ctx A : Typ) (mt : ModTyp) (se1 se2 : Exp) (ce1 ce2 : Core.Exp)
+    : elabExp ctx se1 A ce1
+    → elabExp ctx se2 (Typ.sig (ModTyp.TyArrM A mt)) ce2
+    → elabExp ctx (Exp.mlink se1 se2) (Typ.and A (Typ.sig mt))
+        (Core.Exp.mrg ce1 (Core.Exp.app ce2 ce1))
